compiler/backend/passes/proofs/thunk_untickProofScript.sml
@@ -81,7 +81,7 @@ Inductive exp_rel:
   (∀s vs ws.
      LIST_REL v_rel vs ws ⇒
        v_rel (Constructor s vs) (Constructor s ws)) ∧
-[v_rel_Constructor:]
+[v_rel_Monadic:]
   (∀mop xs ys.
      LIST_REL exp_rel xs ys ⇒
        v_rel (Monadic mop xs) (Monadic mop ys)) ∧
