compiler/backend/languages/semantics/stateLangScript.sml
@@ -1590,6 +1590,6 @@ Termination
   WF_REL_TAC ‘measure cexp_size’
 End
 
-Theorem exp_of_def[simp] = exp_of_def |> CONV_RULE (DEPTH_CONV ETA_CONV);
+Theorem exp_of_def[simp,allow_rebind] = exp_of_def |> CONV_RULE (DEPTH_CONV ETA_CONV);
 
 val _ = export_theory ();
